Properties/Liveness_tla.v
@@ -1,0 +1,663 @@
+From Coq Require Import List Bool Lia ssrbool ListSet Permutation PeanoNat.
+From Coq Require ssreflect.
+Import ssreflect.SsrSyntax.
+From ABCProtocol Require Import Types Address Protocol States Network ListFacts Invariant.
+
+From TLA Require Export logic.
+
+From stdpp Require list.
+
+Module Type ACLiveness 
+  (A : NetAddr) (T : Types A) (AC : ACProtocol A T) (Ns : NetState A T AC)
+  (ACN : ACNetwork A T AC Ns) (ACInv : ACInvariant A T AC Ns ACN).
+
+Import A T AC Ns ACN ACInv.
+
+(* Definition good_deliver_action w w' :=
+  exists p, is_byz (src p) = false /\ In p (sentMsgs w) /\
+    (consumed p = false) /\ (* ? *)
+    system_step (Deliver p) w w'. *)
+(*
+Definition good_deliver_action w w' :=
+  forall p, is_byz (src p) = false -> In p (sentMsgs w) ->
+    (consumed p = false) -> (* ? *)
+    system_step (Deliver p) w w'. 
+*)
+
+Definition satisfies {Σ : Type} (p : predicate Σ) (e : exec Σ) := p e.
+
+#[local] Hint Unfold satisfies : tla.
+
+Notation "e ⊨ p" := (satisfies p%L e) (at level 100).
+
+Definition init w := w = initWorld.
+
+Definition next w w' := ∃ q, system_step q w w'.
+
+#[local] Hint Unfold init next : tla.
+
+Fact is_invariant_in_tla P (H : is_invariant_step P) :
+  ⌜ P ⌝ ∧ □ ⟨next⟩ ⊢ □ ⌜ P ⌝.
+Proof.
+  apply init_invariant; auto.
+  intros ?? HH (q & Hstep).
+  revert HH Hstep.
+  now apply H.
+Qed.
+
+Fact reachable_in_tla :
+  ⌜ init ⌝ ∧ □ ⟨ next ⟩ ⊢ □ ⌜ reachable ⌝.
+Proof.
+  apply init_invariant; autounfold with tla.
+  - intros ? ->.
+    constructor.
+  - intros ??? (q & Hstep).
+    econstructor; eauto.
+  (*
+  autounfold with tla.
+  unfold init, next.
+  intros e (E & H) n.
+  induction n as [ | n IH ].
+  - rewrite drop_0 E.
+    constructor.
+  - specialize (H n).
+    destruct H as (q & H).
+    rewrite ! drop_n in H.
+    simpl in H.
+    econstructor; eauto.
+  *)
+Qed.
+
+(*
+Definition deliver_action_p p w w' :=
+  system_step (Deliver p) w w'.
+*)
+
+(*
+Definition good_deliver_action_p p w w' :=
+  is_byz (src p) = false /\ In p (sentMsgs w) /\
+    (consumed p = false) /\ (* ? *)
+    system_step (Deliver p) w w'.
+*)
+
+(*
+Definition fairness : predicate World :=
+  ∀ p : Packet, 
+    □ (⌜ λ w : World, is_byz (src p) = false ∧ (consumed p = false) ∧ In p (sentMsgs w) ⌝ →
+      weak_fairness (deliver_action_p p)).
+*)
+(*
+(* too strict? *)
+Definition good_deliver_action_p p w w' :=
+  is_byz (src p) = false /\ In p (sentMsgs w) /\
+    (consumed p = false) /\ (* ? *)
+    system_step (Deliver p) w w'.
+*)
+
+Definition good_deliver_action_p p w w' :=
+  is_byz (src p) = false ∧ In p (sentMsgs w) ∧
+    (* if p is already received then underspecify this transition *)
+    (if consumed p then True else system_step (Deliver p) w w').
+
+Definition fairness : predicate World :=
+  ∀ p : Packet, weak_fairness (good_deliver_action_p p).
+
+#[local] Hint Unfold good_deliver_action_p fairness : tla.
+
+Fact psent_persistent_single p :
+  ⌜ λ w, In p (sentMsgs w) ⌝ ∧ □ ⟨ next ⟩ ⊢
+    □ (⌜ λ w, ∃ p', pkt_le p p' ∧ In p' (sentMsgs w) ⌝).
+Proof.
+  unfold pkt_le.
+  apply init_invariant.
+  - intros w Hin.
+    exists p.
+    split; try tauto.
+  - intros w w' (p' & Ep' & Hin) (q & Hstep).
+    (* TODO extract this out? even more troublesome than below! *)
+    inversion Hstep; subst.
+    1,3-6: exists p'; split; try assumption; simpl; auto.
+    1: destruct (procInt _ _) in *; subst; simpl; rewrite in_app_iff; tauto.
+    destruct (procMsgWithCheck _ _ _) in *.
+    subst; cbn delta [sentMsgs] beta iota.
+    destruct (Packet_eqdec p p0) as [ <- | Hneq ].
+    + exists (receive_pkt p).
+      simpl.
+      split; try tauto.
+    + destruct (if Packet_eqdec (receive_pkt p) p0 then (negb (consumed p)) else false) eqn:E0.
+      * destruct (Packet_eqdec (receive_pkt p) p0) as [ <- | ]; try discriminate.
+        apply negb_true_iff in E0.
+        exists (receive_pkt p).
+        split; try tauto.
+        simpl.
+        left; apply receive_pkt_idem.
+      * exists p'.
+        split; try assumption.
+        simpl; rewrite in_app_iff.
+        right; left.
+        apply in_in_remove; try assumption.
+        destruct Ep' as [ <- | Ep' ]; try congruence.
+        subst p'.
+        intros <-.
+        destruct (Packet_eqdec _ _) in E0; try contradiction.
+        apply negb_false_iff, receive_pkt_intact in E0.
+        congruence.
+Qed.
+
+(* certainly, we would like to check whether this is actually what we want! *)
+
+Definition reliable_condition (e : exec World) :=
+  ∀ p, good_packet p → ∀ n, In p (sentMsgs (e n)) →
+    ∃ k, In (receive_pkt p) (sentMsgs (e (k + n))).
+
+Fact fairness_adequate (e : exec World) (Hrc : e ⊨ ⌜ init ⌝ ∧ □ ⟨ next ⟩) :
+  (e ⊨ fairness)%L ↔ reliable_condition e.
+Proof.
+  unfold reliable_condition.
+  autounfold with tla in *.
+  split; intros H. 
+  - intros p Hg n Hin.
+    (* use persistent condition *)
+    unshelve epose proof (psent_persistent_single p (drop n e) (conj Hin _)) as HH.
+    1: unseal. (* ! *)
+    weak_fairness
+
+
+
+    
+
+    destruct (consumed p) eqn:E.
+    + exists 0.
+      simpl.
+      now rewrite (proj1 (receive_pkt_intact p) E).
+    + 
+    
+      specialize (HH p n).
+      epose proof (HH ?[Goalq]) as (k & HH').
+      [Goalq]:{
+        intros k. 
+        hnf.
+        rewrite drop_drop drop_n.
+        simpl.
+        
+        
+        destruct (HH _) as (k & HH).
+      removehead HH. 
+      
+
+
+
+
+      
+  unseal.
+  
+  
+  split.
+  - 
+(*
+Lemma eventual_delivery_single p (Hgood : good_packet p) :
+  □ ⟨ next ⟩ ∧ weak_fairness good_deliver_action ⊢
+  □ ⟨ next ⟩ ∧ weak_fairness (good_deliver_action_p p).
+Proof.
+
+  unseal.
+  destruct H. split; auto.
+  intros. unfold good_deliver_action, good_deliver_action_p in *.
+  specialize (H0 k).
+*)
+
+(* TODO can we do these only at the level of proof modes? this is too ... *)
+(*
+Fact foo1 [Σ : Type] (p1 q1 p2 q2 : predicate Σ)
+  (H1 : p1 ⊢ q1) (H2 : p2 ⊢ q2) : ((p1 ∧ p2) ⊢ (q1 ∧ q2)).
+Proof. autounfold with tla in *. intuition. Qed.
+*)
+(*
+(* not really useful ... *)
+Fact foo2 [Σ : Type] (Γ p1 q1 p2 q2 : predicate Σ)
+  (H1 : Γ ⊢ p1 ~~> □ q1) (H2 : Γ ⊢ p2 ~~> □ q2) : 
+  Γ ⊢ (p1 ∧ p2) ~~> □ (q1 ∧ q2).
+Proof.
+  hnf in H1, H2.
+  unfold leads_to, always, eventually, tla_implies in H1, H2.
+  unseal.
+  destruct H0.
+  specialize (H1 _ H k H0).
+  specialize (H2 _ H k H3).
+  destruct H1 as (k1 & H1), H2 as (k2 & H2).
+  repeat setoid_rewrite drop_drop in H1.
+  repeat setoid_rewrite drop_drop in H2.
+  exists (Nat.max k1 k2).
+  intros kk.
+  split.
+  - now replace (kk + Nat.max k1 k2 + k) with ((kk + Nat.max k1 k2 - k1) + k1 + k) by lia.
+  - now replace (kk + Nat.max k1 k2 + k) with ((kk + Nat.max k1 k2 - k2) + k2 + k) by lia.
+Qed.
+*)
+Fact foo2 [Σ : Type] (Γ p1 q1 p2 q2 : predicate Σ) (next : action Σ)
+  (H1 : □ ⟨ next ⟩ ∧ Γ ⊢ p1 ~~> q1) (H2 : □ ⟨ next ⟩ ∧ Γ ⊢ p2 ~~> q2)
+  (* q1 and q2 have to be persistent *)
+  (* writing H1' and H2' in this way would align with the form of invariant *)
+  (H1' : q1 ∧ □ ⟨ next ⟩ ⊢ □ q1) (H2' : q2 ∧ □ ⟨ next ⟩ ⊢ □ q2) : 
+  □ ⟨ next ⟩ ∧ Γ ⊢ (p1 ∧ p2) ~~> (q1 ∧ q2).
+Proof.
+  autounfold with tla in *.
+  intros.
+  destruct H0.
+  specialize (H1 _ H k H0).
+  specialize (H2 _ H k H3).
+  destruct H1 as (k1 & H1), H2 as (k2 & H2).
+  rewrite ! drop_drop in H1, H2.
+  destruct H.
+  assert (∀ (k k0 : nat), next (drop k (drop k0 e) 0) (drop k (drop k0 e) 1)) as H' 
+    by (intros; now rewrite drop_drop).
+  specialize (H1' _ (conj H1 (fun k => H' k _)) (Nat.max k1 k2 - k1)).
+  specialize (H2' _ (conj H2 (fun k => H' k _)) (Nat.max k1 k2 - k2)).
+  rewrite ! drop_drop in H1', H2'.
+  replace (drop _ e) with (drop (Nat.max k1 k2 + k) e) in H1' by (f_equal; lia).
+  replace (drop _ e) with (drop (Nat.max k1 k2 + k) e) in H2' by (f_equal; lia).
+  repeat setoid_rewrite drop_drop.
+  eauto.
+Qed.
+
+Fact foo2' [A Σ : Type] (Γ : predicate Σ) (p q : A → predicate Σ) (next : action Σ)
+  (* TODO the validity condition is cumbersome! *)
+  (valid : A → Prop)
+  (H : forall (a : A), valid a → (□ ⟨ next ⟩ ∧ Γ ⊢ (p a) ~~> (q a))%L)
+  (H' : forall (a : A), valid a → ((q a) ∧ □ ⟨ next ⟩ ⊢ □ (q a))%L)
+  (l : list A) (Hv : Forall valid l) :
+    (□ ⟨ next ⟩ ∧ Γ ⊢ (fold_right tla_and tla_true (map p l)) ~~> 
+      (fold_right tla_and tla_true (map q l)))%L ∧
+    (* the following needs to be proved together *)
+    ((fold_right tla_and tla_true (map q l)) ∧ □ ⟨next⟩ ⊢
+      (□ fold_right tla_and tla_true (map q l)))%L.
+Proof.
+  induction Hv as [ | a l Ha Hv (IH1 & IH2) ]; simpl.
+  - split.
+    + now apply impl_drop_hyp, impl_to_leads_to.
+    + unseal.
+  - split.
+    + apply foo2; auto.
+    + specialize (H' a).
+      rewrite always_and.
+      tla_split.
+      * etransitivity.
+        2: apply H'; try assumption.
+        tla_assumption.
+      * etransitivity.
+        2: apply IH2.
+        tla_assumption.
+Qed.
+
+Fact foo2'' [A Σ : Type] (Γ : predicate Σ) (p q : A → Σ → Prop) (next : action Σ)
+  (valid : A → Prop)
+  (H : forall (a : A), valid a → (□ ⟨ next ⟩ ∧ Γ ⊢ ⌜ p a ⌝ ~~> ⌜ q a ⌝)%L) 
+  (H' : forall (a : A), valid a → (⌜ q a ⌝ ∧ □ ⟨ next ⟩ ⊢ □ ⌜ q a ⌝)%L)
+  (l : list A) (Hv : Forall valid l) :
+    □ ⟨ next ⟩ ∧ Γ ⊢ 
+      ⌜ λ w, (∀ a, In a l → p a w) ⌝ ~~> ⌜ λ w, (∀ a, In a l → q a w) ⌝.
+Proof.
+  etransitivity.
+  1: apply (proj1 (foo2' _ _ _ _ valid H H' l Hv)).
+  clear Hv.
+  eapply leads_to_weaken.
+  - unseal.
+    rewrite <- Forall_forall in H0.
+    induction H0; simpl; auto.
+  - unseal.
+    revert a H1.
+    rewrite <- Forall_forall.
+    induction l; simpl in H0; auto.
+    constructor; intuition.
+Qed.
+
+(* Fact foo2 [Σ : Type] (Γ p1 q1 p2 q2 : predicate Σ) (next : action Σ)
+  (H1 : □ ⟨ next ⟩ ∧ Γ ⊢ p1 ~~> q1) (H2 : □ ⟨ next ⟩ ∧ Γ ⊢ p2 ~~> q2)
+  (* q1 and q2 have to be persistent *)
+  (* writing H1' and H2' in this way would align with the form of invariant *)
+  (H1' : q1 ∧ □ ⟨ next ⟩ ⊢ □ q1) (H2' : q2 ∧ □ ⟨ next ⟩ ⊢ □ q2) : 
+  □ ⟨ next ⟩ ∧ Γ ⊢ (p1 ∧ p2) ~~> (q1 ∧ q2). *)
+
+(*
+Fact foo3 [Σ : Type] (Γ p q r : predicate Σ) (H : Γ ⊢ q ~~> r) :
+  Γ ⊢ (□ p ∧ q) ~~> (□ p ∧ r).
+Proof.
+  hnf in H.
+  unfold leads_to, always, eventually, tla_implies in H.
+  unseal.
+  destruct H1.
+  specialize (H _ H0 k H2).
+  destruct H as (k1 & H).
+  rewrite drop_drop in H.
+  exists k1.
+  split; auto.
+Qed.
+*)
+(* modus ponens? but with the same hypotheses *)
+(*
+Fact foo4 [Σ : Type] (Γ p q : predicate Σ)
+  (Hp : Γ ⊢ p) (Hpq : Γ ⊢ p → q) : Γ ⊢ q.
+Proof. firstorder. Qed.
+*)
+(* like leads_to_weaken, but with hypotheses *)
+(*
+Fact foo5 [Σ : Type] (Γ p1 p2 q1 q2 : predicate Σ)
+  (H : Γ ⊢ p1 ~~> q1) (Hpre : Γ ⊢ p2 → p1) (Hpost : Γ ⊢ q1 → q2) : 
+  Γ ⊢ p2 ~~> q2.
+Proof. 
+  autounfold with tla in *.
+  intros.
+  apply Hpre in H1.
+*)
+
+(* TODO cannot see better way for now *)
+(*
+Fact psent_persistent pkts :
+  ⌜λ w, incl pkts (sentMsgs w)⌝ ∧ □ ⟨ next ⟩ ⊢
+    □ (⌜λ w, ∃ pkts', Forall2 pkt_le pkts pkts' ∧ incl pkts' (sentMsgs w)⌝).
+Proof.
+  induction pkts as [ | p pkts IH ].
+  - apply impl_drop_hyp.
+    unseal.
+    now exists nil.
+  - pose proof (psent_persistent_single p) as H.
+    match type of IH with pred_impl ?a _ => 
+      match type of H with pred_impl ?b _ => 
+        transitivity (a ∧ b)%L end end.
+    + tla_simp.
+      repeat (tla_split; try tla_assumption).
+      all: apply impl_drop_one, state_pred_impl; intros w.
+      all: unfold incl; simpl; intuition.
+    + etransitivity.
+      1: apply foo1; eassumption.
+      (* degrade *)
+      rewrite <- always_and.
+      apply impl_under_always.
+      rewrite combine_state_preds.
+      apply state_pred_impl.
+      intros w ((pkts' & Ha1 & Ha2) & (p' & Hb1 & Hb2)).
+      exists (p' :: pkts').
+      split.
+      * now constructor.
+      * hnf in Ha2 |- *; simpl. 
+        intros p0 [ <- | Hin ]; intuition.
+Qed.
+*)
+Lemma eventual_delivery_single p (Hgood : good_packet p) :
+  □ ⟨ next ⟩ ∧ fairness ⊢
+  ⌜λ w, In p (sentMsgs w)⌝ ~~> ⌜λ w, In (receive_pkt p) (sentMsgs w)⌝.
+Proof.
+  unfold next, fairness, good_deliver_action_p.
+  evar (bb : predicate World).
+  match goal with |- pred_impl (tla_and ?aa _) _ =>
+    transitivity (tla_and aa bb) end.
+  1: tla_split; [ tla_assumption | ].
+  1: rewrite tla_and_comm; subst bb; apply impl_drop_one, forall_apply with (x0:=p).
+  subst bb.
+  apply wf1.
+  - intros w w' Hin (q & Hstep).
+    (* TODO repeating? *)
+    inversion Hstep; subst.
+    1,3-6: left; simpl; auto.
+    1: destruct (procInt _ _) in *; subst; simpl; rewrite in_app_iff; tauto.
+    destruct (procMsgWithCheck _ _ _) in *.
+    subst; cbn delta [sentMsgs] beta iota.
+    destruct (Packet_eqdec p p0) as [ <- | Hneq ].
+    + right.
+      simpl; now left.
+    + left.
+      simpl; rewrite in_app_iff.
+      right; left.
+      now apply in_in_remove.
+  - intros w w' Hin (q & Hstep') (_ & H_src_nonbyz & Hstep).
+    destruct p as [ ? ? ? [] ].
+    + eapply psent_norevert_is_invariant; eauto.
+    + simpl in Hstep.
+      clear q Hstep'.
+      inversion Hstep; try discriminate.
+      injection H as <-.
+      destruct (procMsgWithCheck _ _ _) in *.
+      subst; cbn; now left.
+  - intros w Hin.
+    hnf in Hgood |- *.
+    destruct Hgood as (? & ? & ? & ?).
+    eexists.
+    split_and ?; try assumption.
+    destruct (consumed p) eqn:EE; try exact I.
+    eapply DeliverStep; eauto.
+    (* ...? *)
+    rewrite (surjective_pairing (procMsgWithCheck _ _ _)).
+    reflexivity.
+Qed.
+(*
+Lemma leads_to_fork' {Σ A: Type} (h: A → Σ → Prop) (h': A → Prop)
+  (f: predicate Σ) (p q: Σ → Prop) :
+  (f ⊢ ⌜p⌝ ~~> ⌜λ s, ∃ x, h' x ∧ h x s⌝) →
+  (∀ (x: A), h' x → (f ⊢ ⌜h x⌝ ~~> ⌜q⌝)) →
+  (f ⊢ ⌜p⌝ ~~> ⌜q⌝).
+Proof.
+  intros Hph Hhq.
+  erewrite <- leads_to_trans; tla_split; [ apply Hph | ].
+  apply leads_to_exist_intro.
+  intros x. unseal. destruct H0. eapply Hhq; try eassumption.
+Qed.
+*)
+Corollary eventual_delivery pkts (Hgood : Forall good_packet pkts) :
+  □ ⟨ next ⟩ ∧ fairness ⊢
+  ⌜λ w, incl pkts (sentMsgs w)⌝ ~~> 
+  ⌜λ w, ∀ p, In p pkts → In (receive_pkt p) (sentMsgs w)⌝. (* need some detour if not to write in this way *)
+Proof.
+  apply foo2'' with (valid:=good_packet); try assumption.
+  - intros; now apply eventual_delivery_single.
+  - intros p _.
+    apply is_invariant_in_tla, psent_norevert_is_invariant.
+Qed.
+
+  (*
+
+  induction pkts as [ | n IH [ | p pkts ] Elen ] using list_ind_3; try discriminate.
+  - simpl.
+    apply impl_drop_hyp, leads_to_refl.
+  - cbn delta [map] beta iota.
+    simpl in Elen.
+    injection Elen as <-.
+    apply Forall_cons_iff in Hgood.
+    destruct Hgood as (Hg & Hgood).
+    (* this is nice *)
+    apply leads_to_fork' with (h':=fun pkts' => Forall2 pkt_le pkts pkts')
+      (h:=fun pkts' w => incl (receive_pkt p :: pkts') (sentMsgs w)).
+    + admit.
+    + intros pkts' Hf.
+      assert (Forall good_packet pkts') as Htmp.
+      { eapply list.Forall2_Forall_r; try eassumption.
+        revert Hgood.
+        apply Forall_impl.
+        intros; rewrite <- pkt_le_good_packet; eauto.
+      }
+      specialize (IH _ (eq_sym (list.Forall2_length _ _ _ Hf)) Htmp).
+      
+
+      (* eapply foo4.
+      1: apply IH. *)
+
+
+      etransitivity.
+      2: apply leads_to_weaken with 
+        (p1:=((□ ⌜ λ w : World, In (receive_pkt p) (sentMsgs w) ⌝) ∧ ⌜ λ w : World, incl pkts' (sentMsgs w) ⌝)%L)
+        (q1:=((□ ⌜ λ w : World, In (receive_pkt p) (sentMsgs w) ⌝) ∧ ⌜ λ w : World, incl (map receive_pkt pkts') (sentMsgs w) ⌝)%L).
+      * now apply foo3.
+      * always state_pred
+      leads_to 
+
+
+    etransitivity.
+    2: apply leads_to_trans with (q:=⌜λ w, ∃ pkts', Forall2 pkt_le pkts pkts' ∧ incl (receive_pkt p :: pkts') (sentMsgs w)⌝).
+    tla_split.
+    + admit.
+    + (* ex elim *)
+      eapply leads_to_fork.
+      rewrite <- exist_state_pred.
+      apply leads_to_exist_intro.
+      intros pkts'.
+      leads_to state_pred tla_and
+      
+  
+    etransitivity.
+    1: apply IH.
+
+
+    leads_to "refl"
+  
+
+
+
+
+Lemma eventual_delivery_single p (Hgood : good_packet p) :
+  □ ⟨ next ⟩ ∧ weak_fairness good_deliver_action ⊢
+  ⌜λ w, In p (sentMsgs w)⌝ ~~> ⌜λ w, In (receive_pkt p) (sentMsgs w)⌝.
+Proof.
+  unfold next.
+  apply wf1.
+  - intros w w' Hin (q & Hstep).
+    (* TODO extract this out? *)
+    inversion Hstep; subst.
+    1,3-6: left; simpl; auto.
+    1: destruct (procInt _ _) in *; subst; simpl; rewrite in_app_iff; tauto.
+    destruct (procMsgWithCheck _ _ _) in *.
+    subst; cbn delta [sentMsgs] beta iota.
+    destruct (Packet_eqdec p p0) as [ <- | Hneq ].
+    + right.
+      simpl; now left.
+    + left.
+      simpl; rewrite in_app_iff.
+      right; left.
+      now apply in_in_remove.
+  - intros w w' Hin _ (p' & H_src_nonbyz & Hin' & Hstep).
+    hnf in Hdl.
+      
+
+
+    1-5: auto.
+    inversion Hstep.
+
+
+Lemma eventual_delivery pkts (Hgood : Forall good_packet pkts) :
+  □ ⟨ next ⟩ ∧ weak_fairness good_deliver_action ⊢
+  ⌜λ w, incl pkts (sentMsgs w)⌝ ~~> ⌜λ w, incl (map receive_pkt pkts) (sentMsgs w)⌝.
+Proof.
+  unfold next.
+  apply wf1.
+  - 
+*)
+
+Lemma bar1 e (H : (□ ⟨ next ⟩)%L e) k o :
+  exists l, system_trace (e k) l ∧ (e (o + k) = final_world (e k) l).
+Proof.
+  autounfold with tla in H.
+  unfold next in H.
+  induction o as [ | o IH ].
+  - now exists nil.
+  - destruct IH as (l & Htrace & Ew0).
+    specialize (H (o + k)).
+    destruct H as (q & Hstep).
+    rewrite ! drop_n in Hstep.
+    simpl in Hstep.
+    exists (l ++ (q, e (S (o + k))) :: nil).
+    rewrite system_trace_app -final_world_app final_world_cons -Ew0 /=.
+    split; auto.
+Qed.
+
+(* one-hop *)
+Lemma bar (P Q : World -> Prop)
+  (H : forall w (Hw : reachable w),
+    (* message-driven *)
+    P w → exists pkts, Forall good_packet pkts ∧ incl pkts (sentMsgs w) ∧
+      (forall w0 l0 (Htrace : system_trace w l0) (Ew0 : w0 = final_world w l0),
+        incl (map receive_pkt pkts) (sentMsgs w0) → Q w0)) :
+  ⌜ init ⌝ ∧ □ ⟨ next ⟩ ∧ fairness ⊢ ⌜ P ⌝ ~~> ⌜ Q ⌝.
+Proof.
+  tla_pose reachable_in_tla.
+  unseal.
+  destruct H0 as (_ & Hnext & Hfair & Hrc).
+  specialize (H (e k) (Hrc _) H1).
+  destruct H as (pkts & Hgood & Hincl & H).
+  pose proof (eventual_delivery _ Hgood e (conj Hnext Hfair) k Hincl) as (k0 & Htmp).
+  exists k0.
+  hnf in Htmp.
+  rewrite drop_drop drop_n /= in Htmp.
+  pose proof (bar1 e Hnext k k0) as (l & Htrace & Ew0).
+  specialize (H _ _ Htrace Ew0).
+  apply H.
+  intros ? (p & <- & ?)%in_map_iff.
+  now apply Htmp.
+Qed.
+
+(* now, really nice things *)
+
+Lemma terminating_convergence_in_tla v (H_byz_minor : num_byz ≤ t0) :
+  ⌜ init ⌝ ∧ □ ⟨ next ⟩ ∧ fairness ⊢
+  ⌜ all_honest_nodes_submitted v ⌝ ~~> ⌜ all_honest_nodes_confirmed ⌝.
+Proof.
+  apply bar.
+  intros.
+  pose proof (honest_submit_all_received_suffcond _ _ Hw H) as Hsuffcond.
+  destruct (submit_msgs_all_sent w v Hw H) as (pkts & Hincl & Hgood & Htmp).
+  simpl in Hsuffcond; clear Htmp.
+  exists pkts.
+  split_and ?; try assumption.
+  intros.
+  eapply terminating_convergence; try eassumption; eauto.
+Qed.
+
+Lemma eventually_accountability_in_tla :
+  ⌜ init ⌝ ∧ □ ⟨ next ⟩ ∧ fairness ⊢
+  ⌜ λ w, ∃ n1 : Address, ∃ n2 : Address, confirmed_different_values n1 n2 w ⌝ ~~> ⌜ accountability ⌝.
+Proof.
+  (* intro first *)
+  let tac n := rewrite <- exist_state_pred; apply leads_to_exist_intro; intros n in tac n1; tac n2.
+  tla_apply (leads_to_trans _ (⌜ mutual_lightcert_conflict_detected n1 n2 ⌝)).
+  tla_split.
+  - apply bar.
+    intros.
+    pose proof (mutual_lightcerts_sent _ _ _ Hw H) as (b1 & b2 & b3 & b4 & Hsuffcond).
+    exists (mutual_lightcerts w n1 n2 b1 b2 b3 b4).
+    change (map receive_pkt _) with (mutual_lightcerts w n1 n2 true true true true).
+    split_and ?; try assumption.
+    1: unfold confirmed_different_values, confirmed in H.
+    1: unfold mutual_lightcerts; repeat (constructor; try tauto).
+    intros.
+    eapply eventually_mutual_lightcert_conflict_detected; try eassumption; eauto.
+  - apply bar.
+    intros.
+    pose proof (fullcerts_all_received_suffcond _ _ Hw H) as Hsuffcond.
+    destruct (fullcerts_all_sent w v Hw H) as (pkts & Hincl & Hgood & Htmp).
+    simpl in Hsuffcond; clear Htmp.
+    exists pkts.
+    split_and ?; try assumption.
+    intros.
+    eapply terminating_convergence; try eassumption; eauto.
+
+
+    pose proof (mutual_lightcerts_sent _ _ _ Hw H) as (b1 & b2 & b3 & b4 & Hsuffcond).
+    exists (mutual_lightcerts w n1 n2 b1 b2 b3 b4).
+    change (map receive_pkt _) with (mutual_lightcerts w n1 n2 true true true true).
+    split_and ?; try assumption.
+    1: unfold confirmed_different_values, confirmed in H.
+    1: unfold mutual_lightcerts; repeat (constructor; try tauto).
+    intros.
+    eapply eventually_mutual_lightcert_conflict_detected; try eassumption; eauto.
+
+
+
+
+
+    pose proof (honest_submit_all_received_ _ _ Hw H) as Hsuffcond.
+    destruct (submit_msgs_all_sent w v Hw H) as (pkts & Hincl & Hgood & Htmp).
+    simpl in Hsuffcond; clear Htmp.
+    exists pkts.
+    split_and ?; try assumption.
+    intros.
+    eapply terminating_convergence; try eassumption; eauto.
+Qed.
+
+End ACLiveness.
